LeanSubst.lean
@@ -1,5 +1,6 @@
 -- This module serves as the root of the `LeanSubst` library.
 -- Import modules here that should be built as part of the library.
+import LeanSubst.Notation
 import LeanSubst.Basic
 import LeanSubst.Map
 import LeanSubst.Reduction
